W_step simulation

theories/IntersectionTypes/Reductions/CM2X_HALT_to_CD_TYP.v
@@ -3,7 +3,7 @@ Require Import Undecidability.CounterMachines.CM2X.
 
 Require Import Undecidability.IntersectionTypes.Util.CD_facts.
 
-Require Import List Relations.
+Require Import List Relations PeanoNat Lia.
 Import ListNotations.
 Import CD (var, app, lam).
 
@@ -13,39 +13,117 @@ Section Argument.
 
 Context (P : Cm2x).
 
+#[local] Notation ZERO := (lam (lam (var 1))).
+#[local] Notation SUCC x := (lam (lam (app (var 0) (ren (funcomp S S) x)))).
+
 (* Scott encoding of nat *)
 Fixpoint enc_nat n :=
   match n with
   | 0 => lam (lam (var 1))
-  | S n => lam (lam (app (var 0) (enc_nat n)))
+  | S n => lam (lam (app (var 0) (enc_nat n))) 
   end.
 
+Definition NONE := lam (lam (var 1)).
+
+Definition many_lam n M := Nat.iter n lam M.
+
+Definition many_app M Ms := fold_left app Ms M.
+
+Compute (many_app (var 0) [(var 1); (var 2); (var 3)]). 
+
+Definition many_subst M Ms := subst (fold_right scons var Ms) M.
+
+(* \a.\b.\W.I *)
+Definition HALT := many_lam 4 (var 0).
+
+Lemma many_subst_lam M Ms : many_subst (lam M) Ms = lam (subst (scons (var 0) (fun x=> ren S (fold_right scons var Ms x))) M).
+Proof. done. Qed.
+
+Notation tm_steps := (CD_facts.steps).
+
+Lemma steps_many_app_many_lam n M Ms : 
+  tm_steps (many_app (many_lam (n + length Ms) M) Ms) (many_subst (many_lam n M) (rev Ms)).
+Proof.
+  elim /rev_ind : Ms M n.
+  { move=> M n /=.
+    have -> : n + 0 = n by lia.
+    rewrite /many_subst /= simpl_tm.
+    by apply: rt_refl. }
+  move=> N Ms IH M n /=.
+  rewrite app_length /= /many_app fold_left_app /= -/(many_app _ _).
+  have -> : n + (length Ms + 1) = (S n) +  length Ms by lia.
+  apply: rt_trans.
+  - apply: stepsAppL. by apply: IH.
+  - rewrite /= many_subst_lam. apply: rt_step. apply: stepRed'.
+    rewrite /many_subst rev_app_distr /= !simpl_tm.
+    apply: ext_subst_tm => - [|x]; first done.
+    by rewrite /= !simpl_tm.
+Qed.
+
+(* select i-th argument *)
 Definition enc_tab i k :=
-  Nat.iter (S k) lam (if (Nat.ltb i k) then var i else var k).
+  many_lam k (if (Nat.ltb i k) then var i else HALT).
 
-Notation tm_steps := (clos_refl_trans tm CD_facts.step).
-
-Lemma enc_tab_spec2 i k Ms N : length Ms = k ->
-  k <= i ->
-  tm_steps (fold_right (fun M2 M1 => app M1 M2) (app (enc_tab i k) N) Ms) N.
+Lemma enc_tab_steps_spec i Ms :
+  tm_steps (many_app (enc_tab i (length Ms)) Ms) (nth i (rev Ms) HALT).
 Proof.
-  ?
+  have := steps_many_app_many_lam 0 (if (Nat.ltb i (length Ms)) then var i else HALT) Ms.
+  congr tm_steps.
+  rewrite /= -rev_length.
+  elim: (rev Ms) i. { by case. }
+  move=> M {}Ms IH [|i]. { done. }
+  rewrite /= -IH /many_subst /=.
+  have ->: Nat.ltb (S i) (S (length Ms)) = Nat.ltb i (length Ms) by done.
+  have -> : (if Nat.ltb i (length Ms) then var (S i) else HALT) =
+    ren S (if Nat.ltb i (length Ms) then var i else HALT).
+  { by case (Nat.ltb i (length Ms)). }
+  by rewrite !simpl_tm.
+Qed.
 
-Lemma enc_tab_spec i k Ms N : length Ms = k ->
-  tm_steps (fold_right (fun M2 M1 => app M1 M2) (app (enc_tab i k) N) Ms ) (nth i Ms N).
+(* encode instruction instr at position i *)
+Definition enc_instr (i : nat) (instr : Instruction) :=
+  match instr with
+  | inc => (* \abw.w (1+i) b (1+a) w *)
+      lam (lam (lam (many_app (var 0) [enc_tab (S i) (length P); var 1; SUCC (var 2); var 0])))
+  | dec j => (* \a. a (\bw.w (1+i) b 0 w) (\a'bw.w j b a' w) *)
+      lam (many_app (var 0) [
+        lam (lam (many_app (var 0) [enc_tab (S i) (length P); var 1; ZERO; var 0]));
+        lam (lam (lam (many_app (var 0) [enc_tab j (length P); var 1; var 2; var 0])))])
+  end.
+
+Lemma iter_plus {X} {f : X -> X} {x : X} n m : Nat.iter (n + m) f x = Nat.iter m f (Nat.iter n f x).
 Proof.
-  elim: Ms k i.
-  { move=> [|?]; last done. rewrite /enc_tab. move=> [|i] _ /=.
-    all: by apply: rt_step; apply: stepRed. }
-  
-  move=> M Ms IH [|k] i /=; first done.
-  move=> [/IH] {}IH.
-  move: i => [|i].
-  - admit.
-  - 
+  elim: m; first by rewrite Nat.add_0_r.
+  move=> m /= <-. by have ->: n + S m = S n + m by lia.
+Qed.
 
+Lemma subst_many_lam sigma n M : subst sigma (many_lam n M) =
+  many_lam n (subst (Nat.iter n (fun sigma=> scons (var 0) (funcomp (ren S) sigma)) sigma) M).
+Proof.
+  elim: n sigma. { done. }
+  move=> n IH sigma. rewrite (iter_plus 1 n) /=. congr lam.
+  by rewrite IH.
+Qed.
 
+Lemma subst_enc_tab sigma i n : subst sigma (enc_tab i n) = enc_tab i n.
+Proof.
+  rewrite /enc_tab.
+  rewrite subst_many_lam. congr many_lam.
+  case E: (Nat.ltb i n); last done.
+  move=> /=. elim: n i E. { done. }
+  move=> n IH [|i] /=. { done. }
+  by move=> /IH ->.
+Qed.
 
+Lemma ren_enc_tab xi i n : ren xi (enc_tab i n) = enc_tab i n.
+Proof. by rewrite ren_as_subst_tm subst_enc_tab. Qed.
+
+Lemma subst_enc_instr sigma i instr : subst sigma (enc_instr i instr) = enc_instr i instr.
+Proof. 
+  case: instr=> >; by rewrite /= !subst_enc_tab.
+Qed.
+
+(* NOT NEEDED? *)
 (* Scott encoding of option *)
 Definition enc_option {X : Type} (e : X -> tm) (o : option X) :=
   match o with
@@ -53,6 +131,100 @@ Definition enc_option {X : Type} (e : X -> tm) (o : option X) :=
   | Some x => lam (lam (app (var 0) (e x)))
   end.
 
+(* NOT NEEDED? *)
 Definition enc_nat3 i a b :=
   lam (app (app (app (var 0) (enc_nat i)) (enc_nat a)) (enc_nat b)).
 
+(* \i.i P0 .. Pn *)
+Definition W := lam (many_app (var 0) (rev (map (fun '(i, instr) => enc_instr i instr) (combine (seq 0 (length P)) P)))).
+
+Lemma subst_many_app sigma M Ms : 
+  subst sigma (many_app M Ms) = many_app (subst sigma M) (map (subst sigma) Ms).
+Proof. Admitted.
+
+Lemma nth_combine_seq {X: Type} {l: list X} {i x d} :
+  nth_error l i = Some x -> nth i (combine (seq 0 (length l)) l) d = (i, x).
+Proof.
+  case: d => ??.
+  rewrite combine_nth. { by rewrite seq_length. }
+  move=> /[dup] ?.
+  rewrite seq_nth. { apply /nth_error_Some. by congruence. }
+  by move=> /(@nth_error_nth X) ->.
+Qed.
+
+Lemma W_tm_steps_enc_instr {i instr} :
+  nth_error P i = Some instr ->
+  tm_steps (app W (enc_tab i (length P))) (enc_instr i instr).
+Proof.
+  move=> Hi.
+  apply: rt_trans. { apply: rt_step. by apply: stepRed'. }
+  rewrite subst_many_app /=.
+  have ? : i < length P. { apply /nth_error_Some. by congruence. }
+  evar (Ms : list tm).
+  have := enc_tab_steps_spec i Ms. subst Ms. congr tm_steps.
+  - congr many_app. congr enc_tab.
+    rewrite map_length rev_length map_length combine_length seq_length. lia.
+  - rewrite map_rev rev_involutive map_map (map_nth' (0, inc)).
+    { rewrite combine_length seq_length. lia. }
+    by rewrite (nth_combine_seq Hi) subst_enc_instr.
+Qed.
+
+Lemma subst_enc_nat sigma n : subst sigma (enc_nat n) = enc_nat n.
+Proof.
+  elim: n sigma. { done. }
+  move=> n IH ? /=. by rewrite IH.
+Qed.
+
+Lemma ren_enc_nat xi n : ren xi (enc_nat n) = enc_nat n.
+Proof. by rewrite ren_as_subst_tm subst_enc_nat. Qed.
+
+Definition W_norm := (ren_enc_nat, ren_enc_tab, subst_enc_nat, subst_enc_tab).
+
+Lemma W_step i a b i' a' b' : CM2X.step P (i, (a, b)) = Some (i', (a', b')) -> 
+  tm_steps 
+    (many_app W [enc_tab i (length P); enc_nat a; enc_nat b; W])
+    (many_app W [enc_tab i' (length P); enc_nat a'; enc_nat b'; W]).
+Proof.
+  rewrite /CM2X.step.
+  case Ei: (nth_error P i) => [instr|] Hinstr; last done.
+  apply: rt_trans.
+  { do 3 apply: stepsAppL. by apply: (W_tm_steps_enc_instr Ei). }
+  case: instr Hinstr {Ei}.
+  - (* case inc *)
+    move=> [<- <- <-] /=.
+    apply: rt_trans. { do 2 apply: stepsAppL. apply: rt_step. by apply: stepRed. }
+    rewrite /= !W_norm.
+    apply: rt_trans. { do 1 apply: stepsAppL. apply: rt_step. by apply: stepRed. }
+    rewrite /= !W_norm.
+    apply: rt_trans. { do 0 apply: stepsAppL. apply: rt_step. by apply: stepRed. }
+    rewrite /= !W_norm.
+    by apply: rt_refl.
+  - (* case dec j *)
+    case: a.
+    + move=> j [<- <- <-] /=.
+      apply: rt_trans. { do 2 apply: stepsAppL. apply: rt_step. by apply: stepRed. }
+      rewrite /= !W_norm.
+      apply: rt_trans. { do 3 apply: stepsAppL. apply: rt_step. by apply: stepRed. }
+      rewrite /= !W_norm.
+      apply: rt_trans. { do 2 apply: stepsAppL. apply: rt_step. by apply: stepRed. }
+      rewrite /= !W_norm.
+      apply: rt_trans. { do 1 apply: stepsAppL. apply: rt_step. by apply: stepRed. }
+      rewrite /= !W_norm.
+      apply: rt_trans. { do 0 apply: stepsAppL. apply: rt_step. by apply: stepRed. }
+      rewrite /= !W_norm.
+      by apply: rt_refl.
+    + move=> j a [<- <- <-] /=.
+      apply: rt_trans. { do 2 apply: stepsAppL. apply: rt_step. by apply: stepRed. }
+      rewrite /= !W_norm.
+      apply: rt_trans. { do 3 apply: stepsAppL. apply: rt_step. by apply: stepRed. }
+      rewrite /= !W_norm.
+      apply: rt_trans. { do 2 apply: stepsAppL. apply: rt_step. by apply: stepRed. }
+      rewrite /= !W_norm.
+      apply: rt_trans. { do 2 apply: stepsAppL. apply: rt_step. by apply: stepRed. }
+      rewrite /= !W_norm.
+      apply: rt_trans. { do 1 apply: stepsAppL. apply: rt_step. by apply: stepRed. }
+      rewrite /= !W_norm.
+      apply: rt_trans. { do 0 apply: stepsAppL. apply: rt_step. by apply: stepRed. }
+      rewrite /= !W_norm.
+      by apply: rt_refl.
+Qed.
